Upgrading Define so that it proves more termination goals. Generates lex. combinations and tries them out, so gets some more ordinary recursions. Gets all iterated primitive recursions. Also has been taught about some operations on words (so recursion from w to w-1w will terminate, for example).
Let me know of any bugs/slowdowns, etc.

src/bool/TypeBasePure.sig
@@ -82,11 +82,11 @@ sig
   (* Support for polytypism *)
 
    val typeValue       : (hol_type -> term option) *
-                         (string * string -> term option)   *
+                         (hol_type -> term option) *
                          (hol_type -> term) -> hol_type -> term
    val tyValue         : (hol_type -> term option) *
-                         (string * string -> term option)   *
-                         (string * string -> term) -> hol_type -> term
+                         (hol_type -> term option) *
+                         (hol_type -> term) -> hol_type -> term
 
    val type_size       : typeBase -> hol_type -> term
    val type_encode     : typeBase -> hol_type -> term
