src/num/termination/TotalDefn.sig
@@ -11,9 +11,17 @@ sig
 
    (* Support for interactive termination proofs *)
 
-   val WF_TAC        : thm list -> tactic
-   val TC_SIMP_CONV  : thm list -> conv
-   val TC_SIMP_TAC   : thm list -> thm list -> tactic
+   val default_WF_thms : thm list ref
+   val default_termination_simps : thm list ref
+
+   val PRIM_WF_TAC   : thm list -> tactic
+   val PRIM_TC_SIMP_CONV  : thm list -> conv
+   val PRIM_TC_SIMP_TAC   : thm list -> tactic
+   val PRIM_WF_REL_TAC    : term quotation -> thm list -> thm list -> tactic
+
+   val WF_TAC        : tactic
+   val TC_SIMP_CONV  : conv
+   val TC_SIMP_TAC   : tactic
    val WF_REL_TAC    : term quotation -> tactic
 
    (* Definitions with automated termination proof support *)
